theories/STyping.v
@@ -479,18 +479,11 @@ Proof.
       * eapply typed_scoped. eauto.
       * rewrite max_pred. reflexivity.
   - forward IHh1 by auto. scope_inv IHh1 hs. destruct hs as [_ hsB].
-    (* The problem is that subst_scoping ignores the level ℓ in the
-      substitution typing.
-      It seems better to just go for an eliminator for Sum and then have
-      resurrection.
-      *)
     eapply subst_scoping with (Ξ := []) (Δ := [ _ ]) in hsB.
     + cbn in hsB. eauto.
     + constructor. 2: constructor.
-      eapply scoping_ptm.
-      eapply typed_scoped in h2.
-      eapply scope_sub. 1: eauto.
-      (* The direction is wrong again! *)
+      rewrite max_pred. eapply scoping_ptm.
+      eapply typed_scoped. eauto.
 Abort.
 
 Lemma meta_conv :
